snapshot

src/Framework/Checking.v
@@ -1633,22 +1633,19 @@ Proof.
   end; eauto.
 Qed.
 
+Lemma cbstep_top_fuel_exposed_inv ρ e j r :
+  cbstep_top_fuel ρ e j r ->
+  to_exposed_cres r.
+Proof. intros. inv H; eauto. Qed.
+
 (* Linking *)
 Definition link f x l1 W1 e1 W2 e2 : cexp :=
   CEfun f l1 [] W1 e1
     (CEletapp x f []
        (CEexp W2 e2)).
 
-(* Cross-language Transformtion Specification *)
-Inductive trans_top (W : web_map) (Γ : vars) : AS.exp -> cexp -> Prop :=
-| Trans_top :
-  forall {e},
-    web_map_spec W Γ e ->
-    trans_top W Γ e (CEexp W e).
-
-Hint Constructors trans_top : core.
-
 (* Cross-language Logical Relations *)
+
 Definition E_top' (P : nat -> AS.wval -> clval -> Prop) (i : nat) (ρ1 : AS.env) (e1 : AS.exp) (ρ2 : cenv) (e2 : cexp) : Prop :=
   forall j1 r1,
     j1 <= i ->
@@ -1687,7 +1684,7 @@ Fixpoint V_top (i : nat) (wv : AS.wval) (cv : clval) {struct i} : Prop :=
                       set_lists xs1 vs1 (M.set f1 (AS.Tag l1 (AS.Vfun f1 ρ1 xs1 e1)) ρ1) = Some ρ3 ->
                       set_lists xs2 vs2 (M.set f2 (CTag l2 W (CVfun f2 ρ2 xs2 e2)) ρ2) = Some ρ4 ->
                       web_map_sound W true ρ3 ρ4 e1 ->
-                      E' V_top W true (i0 - (i0 - j)) ρ3 ρ4 e1
+                      E_top' V_top (i0 - (i0 - j)) ρ3 e1 ρ4 (CEexp W e1)
                 end
 
           | _, _ => False
@@ -1739,12 +1736,13 @@ Proof.
           inv H0; invc.
           destruct (exposed_reflect w0); fcrush.
         }
-        unfold E' in *; intros.
+        unfold E_top' in *; intros.
         edestruct HEV as [j2 [r2 [Hstep HR]]]; eauto.
         inv H0; invc.
         destruct (exposed_reflect w0); try contradiction.
 
-        eexists; eexists; split; eauto.
+        exists j2, r2; split; eauto.
+        eapply cbstep_fuel_cbstep_top_fuel; eauto.
         unfold R' in *.
         destruct r1; destruct r2; auto.
         eapply H; eauto; try lia.
@@ -1765,7 +1763,7 @@ Proof.
         rename w into W.
 
         inv H0; invc.
-        assert (HEV : E' V_top W true (i - (i - j)) ρ3 ρ4 e0).
+        assert (HEV : E_top' V_top (i - (i - j)) ρ3 e0 ρ4 (CEexp W e0)).
         {
           eapply (H5 _ vs1 vs2); eauto.
           eapply V_V_top_Forall; eauto; try lia.
@@ -1774,11 +1772,14 @@ Proof.
         unfold E' in *; intros.
         edestruct HEV as [j2 [r2 [Hstep HR]]]; eauto.
         destruct (exposed_reflect w); try contradiction.
-        eexists; eexists; split; eauto.
+
+        exists j2, r2; split; eauto.
+        eapply cbstep_top_fuel_cbstep_fuel; eauto.
+
         unfold R' in *.
         destruct r1; destruct r2; auto.
         eapply H; eauto; try lia.
-        eapply cbstep_fuel_exposed_inv in Hstep; eauto; fcrush.
+        eapply cbstep_top_fuel_exposed_inv in Hstep; eauto; fcrush.
       * inv Hex.
         eexists; (repeat split; eauto).
         eapply V_V_top_Forall; eauto.
@@ -1813,6 +1814,19 @@ Proof.
     eapply cbstep_fuel_exposed_inv; eauto.
 Qed.
 
+Lemma E_top_E W i ρ1 ρ2 e :
+  E_top i ρ1 e ρ2 (CEexp W e) ->
+  E W true i ρ1 ρ2 e.
+Proof.
+  unfold E, E_top, E', E_top'.
+  intros.
+  edestruct H as [j2 [r2 [Hcbstep HR]]]; eauto.
+  exists j2, r2; split; eauto.
+  - eapply cbstep_top_fuel_cbstep_fuel; eauto.
+  - eapply R_R_top; eauto.
+    eapply cbstep_top_fuel_exposed_inv; eauto.
+Qed.
+
 Definition G_top i Γ1 ρ1 Γ2 ρ2 :=
   wf_cenv ρ2 /\
     refine_env ρ1 ρ2 /\
@@ -1823,9 +1837,9 @@ Definition G_top i Γ1 ρ1 Γ2 ρ2 :=
         M.get x ρ1 = Some v1 /\
           M.get x ρ2 = Some v2 /\
           to_exposed v2 /\
-          V i v1 v2.
+          V_top i v1 v2.
 
-Lemma G_top_wf_env_r i Γ1 ρ1 Γ2 ρ2 :
+Lemma G_top_wf_cenv_r i Γ1 ρ1 Γ2 ρ2 :
   G_top i Γ1 ρ1 Γ2 ρ2 ->
   wf_cenv ρ2.
 Proof. unfold G_top. intros; tauto. Qed.
@@ -1834,6 +1848,11 @@ Lemma G_top_refine_env i Γ1 ρ1 Γ2 ρ2 :
   G_top i Γ1 ρ1 Γ2 ρ2 ->
   refine_env ρ1 ρ2.
 Proof. unfold G_top. intros; tauto. Qed.
+
+Lemma G_top_subset_inv i Γ1 ρ1 Γ2 ρ2 :
+  G_top i Γ1 ρ1 Γ2 ρ2 ->
+  Γ2 \subset Γ1.
+Proof. unfold G_top; intros; tauto. Qed.
 
 Lemma G_top_subset i Γ1 ρ1 Γ2 ρ2 Γ3 Γ4 :
   G_top i Γ1 ρ1 Γ2 ρ2 ->
@@ -1857,8 +1876,9 @@ Proof.
   destruct H as [Hwf [Href [Hs HG]]].
   unfold Ensembles.Included, Ensembles.In, Dom_map in *.
   repeat (split; auto); intros.
-  edestruct HG as [v1' [v2 [Heqv1 [Heqv2 [Hex HV]]]]]; eauto.
-  rewrite Heqv1 in H0; inv H0; eauto.
+  edestruct HG as [v1' [v2 [Heqv1 [Heqv2 [Hex HV]]]]]; eauto; invc.
+  eexists; split; eauto.
+  eapply V_V_top; eauto.
 Qed.
 
 (* W is sound for *every* program trace of an open program e *)
@@ -1879,19 +1899,27 @@ Proof.
   intros; eauto.
 Qed.
 
+Lemma web_map_sound_web_map_sound_top W e :
+  (forall ρ1 ρ2,
+      web_map_sound W true ρ1 ρ2 e) ->
+  web_map_sound_top W e.
+Proof.
+  unfold web_map_sound_top, web_map_sound.
+  intros; eauto.
+Qed.
+
 Definition trans_correct_top e e' :=
   forall i ρ1 ρ2,
     G_top i (AS.occurs_free e) ρ1 (AS.occurs_free e) ρ2 ->
     E_top i ρ1 e ρ2 e'.
 
-Lemma fundamental_property_top W e e' :
-  trans_top W (AS.occurs_free e) e e' ->
+Lemma cexp_compat_top W e :
+  web_map_spec W (AS.occurs_free e) e ->
   web_map_sound_top W e ->
-  trans_correct_top e e'.
+  trans_correct_top e (CEexp W e).
 Proof.
   unfold trans_correct_top.
   intros.
-  inv H.
   eapply E_E_top; eauto.
   eapply fundamental_property; eauto.
   eapply web_map_sound_top_web_map_sound; eauto.
@@ -1904,5 +1932,399 @@ Theorem top W etop:
   trans_correct_top etop (CEexp W etop).
 Proof.
   intros H; intros.
-  eauto using fundamental_property_top, web_map_total.
+  eauto using cexp_compat_top, web_map_total.
+Qed.
+
+(* Linking Preservation *)
+
+Lemma V_top_wf_cval_r {i v1 v2}:
+  V_top i v1 v2 ->
+  wf_cval v2.
+Proof.
+  intros HV.
+  destruct i; simpl in *; fcrush.
+Qed.
+
+Lemma V_top_refine_val {i v1 v2}:
+  V_top i v1 v2 ->
+  refine_val v1 v2.
+Proof.
+  intros HV.
+  destruct i; simpl in *; fcrush.
+Qed.
+
+Lemma V_top_wf_cval_Forall_r {i vs1 vs2} :
+  Forall2 (V_top i) vs1 vs2 ->
+  Forall wf_cval vs2.
+Proof.
+  intros.
+  induction H; auto.
+  constructor; auto.
+  eapply V_top_wf_cval_r; eauto.
+Qed.
+
+Lemma V_top_wf_cres_r {i v1 v2}:
+  V_top i v1 v2 ->
+  wf_cres (CRes v2).
+Proof.
+  intros HV.
+  constructor.
+  eapply V_top_wf_cval_r; eauto.
+Qed.
+
+Lemma V_top_exposed_r {i v1 v2}:
+  V_top i v1 v2 ->
+  to_exposed v2.
+Proof.
+  intros.
+  destruct i; destruct v2;
+    simpl in *; fcrush.
+Qed.
+
+Lemma V_top_exposed_Forall_r {i vs1 vs2} :
+  Forall2 (V_top i) vs1 vs2 ->
+  Forall to_exposed vs2.
+Proof.
+  intros.
+  induction H; auto.
+  constructor; auto.
+  eapply V_top_exposed_r; eauto.
+Qed.
+
+Lemma R_top_wf_cres_l {i r1 r2} :
+  R_top i r1 r2 ->
+  wf_cres r2.
+Proof.
+  unfold R.
+  intros.
+  destruct r1; destruct r2; try contradiction; auto.
+  constructor.
+  eapply V_top_wf_cval_r; eauto.
+Qed.
+
+(* Top-level Inversion Lemmas *)
+Lemma R_top_res_inv_l i v1 r2 :
+  R_top i (AS.Res v1) r2 ->
+  exists v2, r2 = CRes v2 /\ V_top i v1 v2.
+Proof.
+  intros.
+  destruct r2; simpl in *; try contradiction.
+  eexists; split; eauto.
+Qed.
+
+(* Top-level Monotonicity Lemmas *)
+Lemma V_top_mono i :
+  forall {j v1 v2},
+    V_top i v1 v2 ->
+    j <= i ->
+    V_top j v1 v2.
+Proof.
+  intros.
+  eapply V_V_top; eauto.
+  eapply V_top_exposed_r; eauto.
+  eapply V_mono; eauto.
+  eapply V_V_top; eauto.
+  eapply V_top_exposed_r; eauto.
+Qed.
+
+Lemma V_top_mono_Forall {vs1 vs2} i j :
+  Forall2 (V_top i) vs1 vs2 ->
+  j <= i ->
+  Forall2 (V_top j) vs1 vs2.
+Proof.
+  intros H.
+  revert j.
+  induction H; simpl; intros; auto.
+  constructor; eauto.
+  eapply V_top_mono; eauto.
+Qed.
+
+Lemma R_top_mono {r1 r2} i j :
+  R_top i r1 r2 ->
+  j <= i ->
+  R_top j r1 r2.
+Proof.
+  unfold R.
+  intros.
+  destruct r1; auto.
+  destruct r2; auto.
+  eapply V_top_mono; eauto.
+Qed.
+
+Lemma E_top_mono {ρ1 ρ2 e1 e2} i j:
+  E_top i ρ1 e1 ρ2 e2 ->
+  j <= i ->
+  E_top j ρ1 e1 ρ2 e2.
+Proof.
+  unfold E_top, E_top'.
+  intros.
+  destruct (H j1 r1) as [j2 [r2 [Hr2 HR]]]; auto; try lia.
+  exists j2, r2; split; eauto.
+  apply R_top_mono with (i - j1); try lia; auto.
+Qed.
+
+Lemma G_top_mono {Γ1 Γ2 ρ1 ρ2} i j:
+  G_top i Γ1 ρ1 Γ2 ρ2 ->
+  j <= i ->
+  G_top j Γ1 ρ1 Γ2 ρ2.
+Proof.
+  unfold G_top.
+  intros.
+  destruct H as [Hwf [Href [HS HG]]].
+  repeat (split; eauto); intros.
+  edestruct HG as [v1 [v2 [Heqv1 [Heqv2 [Hex HV]]]]]; eauto.
+  eexists; eexists; repeat (split; eauto).
+  apply V_top_mono with i; eauto.
+Qed.
+
+(* Top-level Environment Lemmas *)
+Lemma G_top_get {Γ1 Γ2 i ρ1 ρ2}:
+  G_top i Γ1 ρ1 Γ2 ρ2 ->
+  forall x,
+    (x \in Γ1) ->
+    exists v1 v2,
+      M.get x ρ1 = Some v1 /\
+        M.get x ρ2 = Some v2 /\
+        V_top i v1 v2.
+Proof. unfold G. fcrush. Qed.
+
+Lemma G_top_get_list {i Γ1 ρ1 Γ2 ρ2} :
+  G_top i Γ1 ρ1 Γ2 ρ2 ->
+  forall xs,
+    (FromList xs) \subset Γ1 ->
+    exists vs1 vs2,
+      get_list xs ρ1 = Some vs1 /\
+        get_list xs ρ2 = Some vs2 /\
+        Forall2 (V_top i) vs1 vs2.
+Proof.
+  intros HG xs.
+  intros.
+  induction xs; simpl; intros.
+  - eexists; eexists; repeat split; eauto.
+  - rewrite FromList_cons in H.
+    edestruct (G_top_get HG) as [v1 [v2 [Heqv1 [Heqv2 HV]]]]; eauto.
+
+    edestruct IHxs as [vs1 [vs2 [Heqvs1 [Heqvs2 HVs]]]]; eauto.
+    eapply Included_trans; eauto.
+    apply Included_Union_r.
+
+    rewrite Heqv1.
+    rewrite Heqvs1.
+    rewrite Heqv2.
+    rewrite Heqvs2.
+    exists (v1 :: vs1), (v2 :: vs2); repeat (split; auto).
+Qed.
+
+Lemma G_top_set {i Γ1 ρ1 Γ2 ρ2}:
+  G_top i Γ1 ρ1 Γ2 ρ2 ->
+  forall {x v1 v2},
+    V_top i v1 v2 ->
+    G_top i (x |: Γ1) (M.set x v1 ρ1) (x |: Γ2) (M.set x v2 ρ2).
+Proof.
+  intros.
+  unfold G_top; intros.
+
+  split.
+  eapply wf_cenv_set; eauto.
+  eapply G_top_wf_cenv_r; eauto.
+  eapply V_top_wf_cval_r; eauto.
+
+  split.
+  eapply refine_env_set; eauto.
+  eapply G_top_refine_env; eauto.
+  eapply V_top_refine_val; eauto.
+
+  split.
+  apply Included_Union_compat; auto.
+  apply Included_refl.
+  eapply G_top_subset_inv; eauto.
+
+  intros.
+  destruct (M.elt_eq x0 x); subst.
+  - repeat rewrite M.gss.
+    eexists; eexists; repeat split; eauto.
+    eapply V_top_exposed_r; eauto.
+  - repeat (rewrite M.gso; auto).
+    assert (x0 \in Γ1) by fcrush.
+    edestruct (G_top_get H x0) as [v1' [v2' [Heqv1' [Heqv2' HV]]]]; eauto; invc.
+    eexists; eexists; repeat (split; eauto).
+    eapply V_top_exposed_r; eauto.
+Qed.
+
+Lemma G_top_set_lists {i Γ1 ρ1 Γ2 ρ2}:
+  G_top i Γ1 ρ1 Γ2 ρ2 ->
+  forall {xs vs1 vs2 ρ3 ρ4},
+    Forall2 (V_top i) vs1 vs2 ->
+    set_lists xs vs1 ρ1 = Some ρ3 ->
+    set_lists xs vs2 ρ2 = Some ρ4 ->
+    G_top i (FromList xs :|: Γ1) ρ3 (FromList xs :|: Γ2) ρ4.
+Proof.
+  intros HG xs.
+  assert (HΓ : Γ2 \subset Γ1) by (eapply G_top_subset_inv; eauto).
+  induction xs; simpl; intros.
+  - destruct vs1; try discriminate.
+    destruct vs2; try discriminate.
+    inv H0; inv H1.
+    eapply G_top_subset; eauto.
+    normalize_sets.
+    rewrite Union_Empty_set_neut_l; eauto.
+    apply Included_refl.
+    eapply Included_Union_compat; eauto.
+    apply Included_refl.
+  - destruct vs1; try discriminate.
+    destruct vs2; try discriminate.
+    destruct (set_lists xs vs1 ρ1) eqn:Heq1; try discriminate.
+    destruct (set_lists xs vs2 ρ2) eqn:Heq2; try discriminate.
+    inv H; inv H0; inv H1.
+    eapply G_top_subset with (Γ1 := (a |: (FromList xs :|: Γ1))) (Γ2 := (a |: (FromList xs :|: Γ2))); eauto.
+    eapply G_top_set; eauto.
+    normalize_sets.
+    rewrite Union_assoc.
+    apply Included_refl.
+    eapply Included_Union_compat; eauto.
+    apply Included_refl.
+Qed.
+
+(* well_annotated is strictly stronger than trans_correct_top *)
+Lemma trans_correct_top_trans_correct W e :
+  web_map_sound_top W e ->
+  trans_correct_top e (CEexp W e) ->
+  well_annotated W (AS.occurs_free e) e.
+Proof.
+  unfold trans_correct_top, well_annotated.
+  intros.
+Abort.
+
+Lemma Vfun_V_top W l w e :
+  W ! l = Some w ->
+  (w \in Exposed) ->
+  trans_correct_top e (CEexp W e) ->
+  forall i f xs Γ1 Γ2 ρ1 ρ2,
+    G_top i Γ1 ρ1 Γ2 ρ2 ->
+    AS.occurs_free e \subset (FromList xs :|: (f |: Γ1)) ->
+    V_top i (AS.Tag l (AS.Vfun f ρ1 xs e)) (CTag l W (CVfun f ρ2 xs e)).
+Proof.
+  unfold trans_correct_top.
+  intros HW Hw He i.
+
+  induction i; simpl; intros; auto;
+    assert (Hρ2 : wf_cenv ρ2) by (eapply G_top_wf_cenv_r; eauto);
+    assert (Hwf : wf_cval (CTag l W (CVfun f ρ2 xs e))) by eauto;
+    assert (Href : refine_val (AS.Tag l (AS.Vfun f ρ1 xs e)) (CTag l W (CVfun f ρ2 xs e))) by eauto using G_top_refine_env;
+    repeat (split; eauto); intros.
+  apply (He (i - (i - j)) ρ3 ρ4); auto.
+  eapply G_top_subset with (Γ1 := FromList xs :|: (f |: Γ1)) (Γ2 := FromList xs :|: (f |: Γ2)); eauto.
+  eapply G_top_set_lists; eauto.
+  eapply G_top_set; eauto.
+  eapply G_top_mono; eauto; try lia.
+  apply V_top_mono with i; try lia.
+  eapply IHi with (Γ2 := Γ2); eauto.
+  apply G_top_mono with (S i); eauto; lia.
+  eapply Included_refl; eauto.
+Qed.
+
+Lemma fun_compat_top W w e k k' f l xs :
+  W ! l = Some w ->
+  (w \in Exposed) ->
+  trans_correct_top e (CEexp W e) ->
+  trans_correct_top k k' ->
+  trans_correct_top (AS.Efun f l xs e k) (CEfun f l xs W e k').
+Proof.
+  unfold trans_correct_top, E_top, E_top'.
+  intros HW Hw; intros.
+
+  inv H3.
+  - exists 0, COOT; split; simpl; eauto.
+  - inv H4.
+    edestruct (H0 (i - 1) (M.set f (AS.Tag l (AS.Vfun f ρ1 xs e)) ρ1) (M.set f (CTag l W (CVfun f ρ2 xs e)) ρ2)) with (j1 := c) (r1 := r1) as [j2 [r2 [Hk2 Rr]]]; eauto; try lia.
+    + eapply G_top_subset with (Γ1 := (f |: (AS.occurs_free (AS.Efun f l xs e k)))); eauto.
+      * eapply G_top_set; eauto.
+        eapply G_top_mono; eauto; try lia.
+
+        eapply Vfun_V_top; eauto.
+        -- eapply G_top_mono; eauto; try lia.
+        -- eapply AS.free_fun_e_subset; eauto.
+      * eapply AS.free_fun_k_subset; eauto.
+      * eapply Included_refl; eauto.
+    + exists (S j2), r2; split; eauto.
+      * constructor; auto.
+        econstructor; eauto.
+        inv Hk2; auto.
+      * apply R_top_mono with ((i - 1) - c); try lia; auto.
+Qed.
+
+
+(* TODO: at the top level, labeling pass should link with the trivial label *)
+
+Lemma preserves_linking W1 W2 f w l1 l2 x e1 e2 :
+  W1 ! l1 = Some w ->
+  (w \in Exposed) ->
+  trans_correct_top e1 (CEexp W1 e1) ->
+  trans_correct_top e2 (CEexp W2 e2) ->
+  trans_correct_top (AS.link f x l1 e1 l2 e2) (link f x l1 W1 e1 W2 e2).
+Proof.
+  unfold AS.link, link.
+  intros.
+  eapply fun_compat_top; eauto.
+  (* eapply letapp_compat_top; eauto. *)
+Abort.
+
+
+Lemma letapp_compat_top k k' l xs x f :
+  trans_correct_top k k' ->
+  trans_correct_top (AS.Eletapp x f l xs k) (CEletapp x f xs k').
+Proof.
+  unfold trans_correct_top, E_top, E_top'.
+  intros.
+
+  inv H2.
+  - exists 0, COOT; split; simpl; auto.
+  - inv H3.
+    + edestruct (G_top_get H0) as [fv1 [fv2 [Heqfv1 [Heqfv2 HVf]]]]; eauto.
+      invc.
+      destruct fv2.
+      destruct i.
+      fcrush.
+      simpl in HVf.
+      rename w into W'.
+      destruct HVf as [Hfv2 [Href [Hexf2 [Heql HV]]]]; subst.
+      destruct c; try contradiction.
+      destruct HV as [Heqf [Heqxs [Heqe HV]]]; subst.
+
+      edestruct (G_top_get_list H0 xs) as [vs1 [vs2 [Heqvs1 [Heqvs2 HVvs]]]]; eauto.
+      eapply AS.free_letapp_xs_subset; eauto.
+
+      invc.
+
+      destruct (set_lists_length3 (M.set v0 (CTag l0 W' (CVfun v0 t l1 e0)) t) l1 vs2) as [ρ4 Heqρ4].
+      unfold clval in *.
+      rewrite <- (Forall2_length _ _ _ HVvs).
+      rewrite <- (set_lists_length_eq _ _ _ _ H12); auto.
+
+      unfold E' in HV.
+      edestruct (HV i vs1 vs2 ρ'' ρ4) with (j1 := c0) as [j2 [r2 [He0 HR]]]; eauto; try lia.
+      * eapply V_top_exposed_Forall_r; eauto.
+      * eapply V_top_mono_Forall; eauto; lia.
+      * admit.
+      * destruct r2; simpl in HR; try contradiction.
+        edestruct (H0 (i - c0) (M.set x v ρ1) (M.set x w ρ2)) with (j1 := c') as [j3 [r3 [He1 HR']]]; eauto; try lia.
+        eapply G_top_subset with (Γ1 := x |: (A0.occurs_free (A0.Eletapp x f xs k))) (Γ2 := x |: (A1.occurs_free (A1.Eletapp x f w0 xs k'))); eauto.
+        eapply G_top_set; eauto.
+        eapply G_top_mono; eauto; lia.
+        -- eapply V_top_mono; eauto; try lia.
+        -- eapply A0.free_letapp_k_subset; eauto.
+        -- exists (S (j2 + j3)), r3; split; eauto.
+           2 : { eapply R_top_mono; eauto; lia. }
+
+           constructor; auto.
+           eapply BStep_letapp_Res with (v := w); eauto.
+           destruct (exposed_reflect w0); try contradiction; auto.
+
+           intros.
+           split; auto.
+           eapply V_top_exposed_Forall_r; eauto.
+           assert (Hw : exposed_res (A1.Res w)) by (eapply bstep_fuel_exposed_inv; eauto); inv Hw; auto.
+
+           eapply bstep_fuel_exposed_inv; eauto.
+    + eexists; exists OOT; split; simpl; eauto.
 Qed.
